src/Std/Tactic/BVDecide/Bitblast/BVExpr/Circuit/Impl/Expr.lean
@@ -240,7 +240,12 @@ where
           apply AIG.LawfulVecOperator.le_size_of_le_aig_size (f := bitblast.blastCpop)
           omega
         ⟨⟨res, this⟩, cache.cast (AIG.LawfulVecOperator.le_size (f := bitblast.blastCpop) ..)⟩
-      | .sqrt => sorry
+      | .sqrt =>
+        let res := bitblast.blastSqrt eaig evec
+        have := by
+          apply AIG.LawfulVecOperator.le_size_of_le_aig_size (f := bitblast.blastSqrt)
+          omega
+        ⟨⟨res, this⟩, cache.cast (AIG.LawfulVecOperator.le_size (f := bitblast.blastSqrt) ..)⟩
     | .append lhs rhs h =>
       let ⟨⟨⟨aig, lhs⟩, hlaig⟩, cache⟩ := goCache aig lhs cache
       let ⟨⟨⟨aig, rhs⟩, hraig⟩, cache⟩ := goCache aig rhs cache
@@ -352,12 +357,11 @@ theorem go_decl_eq (aig : AIG BVBit) (expr : BVExpr w) (cache : Cache aig) :
         · apply Nat.le_trans <;> assumption
   next op expr =>
     match op with
-    | .not | .rotateLeft .. | .rotateRight .. | .arithShiftRightConst .. | .reverse | .clz | .cpop =>
+    | .not | .rotateLeft .. | .rotateRight .. | .arithShiftRightConst .. | .reverse | .clz | .cpop | .sqrt=>
       rw [AIG.LawfulVecOperator.decl_eq]
       rw [goCache_decl_eq]
       have := (goCache aig expr cache).result.property
       exact Nat.lt_of_lt_of_le h1 this
-    | .sqrt => sorry
   next lhsExpr rhsExpr h =>
     have hl := (goCache aig lhsExpr cache).result.property
     have hr := (goCache (goCache aig lhsExpr cache).1.1.aig rhsExpr (goCache aig lhsExpr cache).cache).result.property
